Freigen/ITree/Basic.lean
@@ -1,0 +1,351 @@
+import Freigen.IxPoly.Basic
+
+namespace Freigen.ITree
+
+open Freigen.IxPoly
+
+structure EffSpec where
+  tag : Type u
+  input : tag → Type v
+  output : tag → Type v
+  blockTag : tag → Type u
+  blockInputs : (t : tag) → blockTag t → Type v
+  blockOutputs : (t : tag) → blockTag t → Type v
+
+inductive NodeTag (E : EffSpec) : Type _ → Type _ where
+| ret {R} : R → NodeTag E R
+| tau {R} : NodeTag E R
+| fail {R} : NodeTag E R
+| op {R} (e : E.tag) : E.input e → NodeTag E R
+
+def NodeTag.fields {i} {E : EffSpec}: NodeTag E i → Type _
+| ret _ => PEmpty
+| tau => PUnit
+| fail => PEmpty
+| op e _ => E.output e ⊕ ((t : E.blockTag e) × E.blockInputs e t)
+
+def NodeTag.elem {E : EffSpec} {α : Type _} : (t : NodeTag E α) → (p : t.fields) → Type _
+| ret _, x => nomatch x
+| fail, x => nomatch x
+| tau, () => α
+| op _ _, Sum.inl _ => α
+| op e _, Sum.inr ⟨o, _⟩ => E.blockOutputs e o
+
+def Step (E : EffSpec) : Endo (Type _) where
+  Tag := fun α => NodeTag E α
+  Field := fun _=> NodeTag.fields
+  Elem := fun _ => NodeTag.elem
+
+namespace Step
+
+def ret {E α Y} (x : α) : Step E Y α := ⟨.ret x, fun a => PEmpty.elim a⟩
+def tau {E α Y} (x : Y α) : Step E Y α := ⟨.tau, fun () => x⟩
+def fail {E α Y} : Step E Y α := ⟨.fail, fun a => PEmpty.elim a⟩
+def op {E α Y} (e : E.tag) (inp : E.input e)
+    (blocks : (t : E.blockTag e) → E.blockInputs e t → Y (E.blockOutputs e t))
+    (k : (o : E.output e) → Y α) : Step E Y α :=
+  ⟨.op e inp, fun
+    | Sum.inl o => k o
+    | Sum.inr ⟨t, i⟩ => blocks t i
+  ⟩
+
+protected def casesOn {E Y} { motive : (α : Type _) → Step E Y α → Sort* } {α} (x : Step E Y α)
+    (ret : ∀ {α} x, motive α (ret x))
+    (tau : ∀ {α} x, motive α (tau x))
+    (fail : ∀ {α}, motive α fail)
+    (op : ∀ {α} e inp blocks k, motive α (op e inp blocks k)):
+    motive α x := by
+  rcases x with ⟨tag, fields⟩
+  cases tag with
+  | ret a =>
+    convert ret a
+    simp only [Step.ret]
+    congr 2
+    ext a; cases a
+  | tau =>
+    convert tau (fields ())
+    · rfl
+    · simp only [Step.tau]
+      congr
+  | fail =>
+    convert fail
+    simp only [Step.fail]
+    congr 2
+    ext a; cases a
+  | op e inp =>
+    convert op e inp (fun t i => fields (.inr ⟨t, i⟩)) (fun o => fields (.inl o))
+    simp only [Step.op]
+    congr 2
+    ext a; cases a <;> rfl
+
+@[simp]
+theorem map_ret {E} {Y Z : Type _ → Type _} {f : (α : Type _) → Y α → Z α} {α : Type _} {x : α}:
+    IxPoly.map (F := Step E) f α (Step.ret x) = Step.ret x := by
+  simp only [map, ret]
+  congr 1
+  ext a; cases a
+
+@[simp]
+theorem map_tau {E} {Y Z : Type _ → Type _} {f : (α : Type _) → Y α → Z α} {α : Type _} {x : Y α}:
+    IxPoly.map (F := Step E) f α (Step.tau x) = Step.tau (f α x) := by
+  simp only [map, tau]
+  congr 1
+
+@[simp]
+theorem map_fail {E} {Y Z : Type _ → Type _} {f : (α : Type _) → Y α → Z α} {α : Type _}:
+    IxPoly.map (F := Step E) f α (Step.fail) = Step.fail := by
+  simp only [map, fail]
+  congr 1
+  ext a; cases a
+
+@[simp]
+theorem map_op {E} {Y Z : Type _ → Type _} {f : (α : Type _) → Y α → Z α} {α : Type _}
+    {e : E.tag} {inp : E.input e}
+    {blocks : (t : E.blockTag e) → E.blockInputs e t → Y (E.blockOutputs e t)}
+    {k : (o : E.output e) → Y α}:
+    IxPoly.map (F := Step E) f α (Step.op e inp blocks k) =
+      Step.op e inp (fun t i => f _ (blocks t i)) (fun o => f _ (k o)) := by
+  simp only [map, op]
+  congr 1
+  ext a; cases a <;> rfl
+
+end Step
+
+end ITree
+
+def ITree (E : ITree.EffSpec) (α : Type _): Type _ := (ITree.Step E).M α
+
+namespace ITree
+
+open IxPoly
+
+def corec {E} {A : Type _ → Type _} (f : (i : Type _) → A i → Step E A i): {i : Type _} → A i → ITree E i :=
+  IxPoly.M.corec f
+
+def observe {E α} : ITree E α ≃ Step E (ITree E) α := IxPoly.M.observe
+
+def roll {E α} : Step E (ITree E) α → ITree E α := IxPoly.M.observe.symm
+
+theorem observe_roll {E α} (x : Step E (ITree E) α): observe (roll x) = x := observe.apply_symm_apply _
+
+theorem roll_observe {E α} (x : ITree E α): roll (observe x) = x := observe.symm_apply_apply _
+
+theorem observe_corec {E} {A : Type _ → Type _} (f : (i : Type _) → A i → Step E A i) {i : Type _} (a : A i):
+    observe (corec f a) = IxPoly.map (fun _ y => corec f y) i (f i a) := IxPoly.M.observe_corec
+
+def ret {E α} (x : α) : ITree E α := roll $ Step.ret x
+def tau {E α} (x : ITree E α) : ITree E α := roll $ Step.tau x
+def fail {E α} : ITree E α := roll $ Step.fail
+def op {E α} (e : E.tag) (inp : E.input e)
+    (blocks : (t : E.blockTag e) → E.blockInputs e t → ITree E (E.blockOutputs e t))
+    (k : (o : E.output e) → ITree E α) : ITree E α :=
+  roll $ Step.op e inp blocks k
+
+@[simp]
+theorem observe_tau {E α} (x : ITree E α): observe (tau x) = Step.tau x := by
+  simp only [tau, observe_roll, Step.tau]
+
+protected def casesOn {E} { motive : (α : Type _) → ITree E α → Sort* } {α} (x : ITree E α)
+    (ret : ∀ {α} x, motive α (ret x))
+    (tau : ∀ {α} x, motive α (tau x))
+    (fail : ∀ {α}, motive α fail)
+    (op : ∀ {α} e inp blocks k, motive α (op e inp blocks k)):
+    motive α x := by
+  have : x = roll (observe x) := (observe.symm_apply_apply _).symm
+  rw [this]
+  cases observe x using Step.casesOn <;> apply_assumption
+
+inductive BisimRelF {E}
+    (R : (α : Type _) → ITree E α → ITree E α → Prop):
+    (α : Type _) → Step E (ITree E) α → Step E (ITree E) α → Prop where
+| ret {α} (x : α): BisimRelF R α (Step.ret x) (Step.ret x)
+| tau {α} (x y : ITree E α) (hr : R _ x y) : BisimRelF R α (Step.tau x) (Step.tau y)
+| fail {α} : BisimRelF R α Step.fail Step.fail
+| op {α} (e : E.tag) (inp : E.input e)
+    (k1 k2 : (o : E.output e) → ITree E α)
+    (blocks1 blocks2 : (t : E.blockTag e) → E.blockInputs e t → ITree E (E.blockOutputs e t))
+    (h1 : ∀ o, R _ (k1 o) (k2 o))
+    (h2 : ∀ t i, R _ (blocks1 t i) (blocks2 t i)):
+  BisimRelF R α (Step.op e inp blocks1 k1) (Step.op e inp blocks2 k2)
+
+theorem BisimRelF.toLiftR {E} {R : (α : Type _) → ITree E α → ITree E α → Prop} : BisimRelF R ≤ IxPoly.M.LiftR (Step E) R := by
+  intro α x y hxy
+  cases hxy <;> constructor
+  case ret | fail => intro a; cases a
+  case tau => intro _; assumption
+  case op =>
+    intro a
+    cases a <;> apply_assumption
+
+theorem BisimRelF.refl {E R}
+    (hrefl : ∀ {α} (x : ITree E α), R α x x)
+    {α} (x : Step E (ITree E) α): BisimRelF R α x x := by
+  cases x using Step.casesOn <;> constructor <;> intros <;> apply_assumption
+
+theorem BisimRelF.refl_upToEq {E R}
+    {α} (x : Step E (ITree E) α): BisimRelF (M.IxRel.upToEq R) α x x := by
+  apply BisimRelF.refl
+  intros
+  apply Or.inl
+  rfl
+
+theorem bisim {E α} (R : (α : Type _) → ITree E α → ITree E α → Prop)
+    (step : ∀{α x y}, R α x y → BisimRelF R α (observe x) (observe y))
+    {x y : ITree E α} (hxy : R _ x y) : x = y := by
+  apply IxPoly.M.Bisim.coind (R := R)
+  · intro α x y hxy
+    apply BisimRelF.toLiftR
+    apply step hxy
+  · assumption
+
+theorem bisim_up_to_eq {E α} (R : (α : Type _) → ITree E α → ITree E α → Prop)
+    (step : ∀{α x y}, R α x y → BisimRelF (M.IxRel.upToEq R) α (observe x) (observe y))
+    {x y : ITree E α} (hxy : R _ x y) : x = y := by
+  apply bisim (R := M.IxRel.upToEq R)
+  · intro _ x y hxy
+    cases hxy
+    · rename_i h
+      cases h
+      apply BisimRelF.refl_upToEq
+    · apply step
+      assumption
+  · right
+    assumption
+
+theorem bisim₂ {E α} {Seed : Type _ → Type _}
+    (left right : (i : Type _) → Seed i → ITree E i)
+    (step : ∀ {i} (s : Seed i), BisimRelF (M.IxRel.span Seed left right) i (observe (left i s)) (observe (right i s)))
+    (seed : Seed α): left α seed = right α seed := by
+  apply bisim (R := M.IxRel.span Seed left right)
+  intro i x y hxy
+  rcases hxy with ⟨s, rfl, rfl⟩
+  apply step
+  exists seed
+
+theorem bisim₂_up_to_eq {E α} {Seed : Type _ → Type _}
+    (left right : (i : Type _) → Seed i → ITree E i)
+    (step : ∀ {i} (s : Seed i), BisimRelF (M.IxRel.upToEq (M.IxRel.span Seed left right)) i (observe (left i s)) (observe (right i s)))
+    (seed : Seed α): left α seed = right α seed := by
+  apply bisim_up_to_eq (R := M.IxRel.span Seed left right)
+  intro i x y hxy
+  rcases hxy with ⟨s, rfl, rfl⟩
+  apply step
+  exists seed
+
+def BindCarrier E α R := (ITree E α × (α → ITree E R)) ⊕ ITree E R
+def bindCo {E α} R : BindCarrier E α R → Step E (BindCarrier E α) R
+| .inl (e, f) => match e.observe with
+  | ⟨.ret x, _⟩ => IxPoly.map (fun _ => .inr) _ (f x).observe
+  | ⟨.tau, cont⟩ => ⟨.tau, fun () => .inl (cont (), f)⟩
+  | ⟨.fail, _⟩ => ⟨.fail, fun x => PEmpty.elim x⟩
+  | ⟨.op e x, cont⟩ => ⟨.op e x, fun
+    | .inl o => .inl (cont $ .inl o, f)
+    | .inr b => .inr (cont $ .inr b)
+  ⟩
+| .inr e => IxPoly.map (fun _ => .inr) _ e.observe
+
+theorem bindCo_copy {E β} {x : ITree E β} : corec (bindCo (α := α)) (.inr x) = x := by
+  apply bisim (R := fun _ x y => x = corec (bindCo (α := α)) (.inr y))
+  intro _ x y hxy
+  cases hxy
+  · simp only [observe_corec, bindCo, IxPoly.map_map]
+    cases y.observe using Step.casesOn <;> {
+       try simp; constructor <;> { intros ; apply_assumption }
+    }
+  · rfl
+
+instance {E} : Monad (ITree E) where
+  pure := fun x => ret x
+  bind {α β} (a : ITree E α) (f : α → ITree E β) := corec bindCo (.inl (a, f))
+
+@[simp]
+theorem ret_bind {E β} {α} {x : α} {f : α → ITree E β} : ret x >>= f = f x := by
+  apply observe.injective
+  simp only [Bind.bind, observe_corec, bindCo, ret,
+    observe_roll, IxPoly.map_map, Step.ret, bindCo_copy, IxPoly.map_id]
+
+@[simp]
+theorem tau_bind {E β} {α} {x : ITree E α} {f : α → ITree E β} : tau x >>= f = tau (x >>= f) := by
+  apply observe.injective
+  simp only [Bind.bind, observe_corec, bindCo, tau, observe_roll, Step.tau, IxPoly.map]
+  congr
+
+@[simp]
+theorem fail_bind {E β} {α} {f : α → ITree E β} : fail >>= f = fail := by
+  apply observe.injective
+  simp only [Bind.bind, observe_corec, bindCo, fail, observe_roll, Step.fail, IxPoly.map]
+  congr
+  ext a
+  cases a
+
+@[simp]
+theorem op_bind {E β} {α} {e : E.tag} {inp : E.input e}
+    {blocks : (t : E.blockTag e) → E.blockInputs e t → ITree E (E.blockOutputs e t)}
+    {k : (o : E.output e) → ITree E α}
+    {f : α → ITree E β}:
+    (op e inp blocks k) >>= f =
+      op e inp
+        blocks
+        (fun o => k o >>= f) := by
+  apply observe.injective
+  simp only [Bind.bind, observe_corec, bindCo, op, observe_roll, IxPoly.map]
+  simp only [Step.op]
+  congr
+  ext a; cases a
+  · rfl
+  · simp [bindCo_copy]
+
+inductive BindPureRel {E} : (α: Type _) → ITree E α → ITree E α → Prop where
+| root {α} (m : ITree E α) : BindPureRel α (m >>= pure) m
+| refl {α} (m : ITree E α) : BindPureRel α m m
+
+theorem bind_pure {E α} (a : ITree E α) : a >>= pure = a := by
+  apply bisim₂_up_to_eq (Seed := ITree E) (left := fun _ x => x >>= pure) (right := fun _ x => x)
+  intro _ m
+  cases m using ITree.casesOn with
+  | ret | fail => simp [pure, BisimRelF.refl_upToEq]
+  | tau x =>
+    simp only [tau_bind, observe_tau]
+    apply BisimRelF.tau
+    right
+    exists x
+  | op e inp blocks k =>
+    simp only [op_bind]
+    apply BisimRelF.op
+    · intro
+      right
+      apply Exists.intro
+      apply And.intro <;> rfl
+    · intros; left; rfl
+
+theorem bind_assoc {E α β γ} {a : ITree E α} {f : α → ITree E β} {g : β → ITree E γ}:
+    (a >>= f) >>= g = a >>= fun x => f x >>= g := by
+  apply bisim₂_up_to_eq (Seed := fun γ => ITree E α × (α → ITree E β) × (β → ITree E γ))
+    (left := fun _ ⟨x, f, g⟩ => (x >>= f) >>= g)
+    (right := fun _ ⟨x, f, g⟩ => x >>= fun y => f y >>= g)
+    (seed := ⟨a, f, g⟩)
+  intro _ ⟨x, f, g⟩
+  simp only
+  cases x using ITree.casesOn with
+  | ret | fail => simp [BisimRelF.refl_upToEq]
+  | tau x =>
+    simp only [tau_bind, observe_tau]
+    apply BisimRelF.tau
+    right
+    exists ⟨x, f, g⟩
+  | op e inp blocks k =>
+    simp only [op_bind]
+    apply BisimRelF.op
+    · intro o
+      right
+      exists ⟨k o, f, g⟩
+    · intros; left; rfl
+
+instance {E} : LawfulMonad (ITree E) := LawfulMonad.mk' _
+  bind_pure
+  (fun _ _ => ret_bind)
+  (fun _ _ _ => bind_assoc)
+
+
+
+end Freigen.ITree
